exp.lean
@@ -2,12 +2,7 @@ import data.set
 
 open set
 
-inductive exp₁ : set ℕ → Type :=
-  | var : Π      x,                   exp₁ '{x}
-  | app : Π {X Y} , exp₁ X → exp₁ Y → exp₁ (X ∪ Y)
-  | lam : Π {X}  x, exp₁ X          → exp₁ (X \ '{x})
-
-inductive exp₂ : set ℕ → Type :=
-  | var : Π {X}  x, x ∈ X             → exp₂ X
-  | app : Π {X}   , exp₂ X → exp₂ X   → exp₂ X
-  | lam : Π {X}  x, exp₂ (insert x X) → exp₂ X
+inductive exp : set ℕ → Type :=
+  | var : Π {X}  x, x ∈ X            → exp X
+  | app : Π {X}   , exp X → exp X    → exp X
+  | lam : Π {X}  x, exp (insert x X) → exp X
